LogicalRefinement/Typed/Downgrade.lean
@@ -1,0 +1,175 @@
+import LogicalRefinement.Untyped
+import LogicalRefinement.Untyped.Subst
+import LogicalRefinement.Utils
+import LogicalRefinement.Tactics
+import LogicalRefinement.Typed.Context
+import LogicalRefinement.Typed.Basic
+import LogicalRefinement.Typed.Wk
+import LogicalRefinement.Typed.Subst
+open Term
+open Annot
+open AnnotSort
+
+set_option maxHeartbeats 10000000
+
+theorem HasType.downgrade_helper {Δ Γ: Context} {a A s}
+  : (Δ ⊢ a: A) -> (Γ.is_sub Δ) -> (A = sort s) -> Γ ⊢ a: sort s
+  := by {
+    intro H;
+    induction H generalizing s Γ with
+    | pi HA HB IA IB => 
+      intro HΓΔ Hs;
+      rw [<-Hs]
+      constructor
+      apply IA
+      assumption
+      rfl
+      apply IB
+      constructor
+      assumption
+      constructor
+      constructor
+      rfl
+    | sigma HA HB IA IB => 
+      intro HΓΔ Hs;
+      rw [<-Hs]
+      constructor
+      apply IA
+      assumption
+      rfl
+      apply IB
+      constructor
+      assumption
+      constructor
+      constructor
+      rfl
+    | coprod HA HB IA IB => 
+      intro HΓΔ Hs;
+      rw [<-Hs]
+      constructor
+      apply IA
+      assumption
+      rfl
+      apply IB
+      assumption
+      rfl
+    | set HA HB IA IB => 
+      intro HΓΔ Hs;
+      rw [<-Hs]
+      constructor
+      apply IA
+      assumption
+      rfl
+      apply IB
+      constructor
+      assumption
+      constructor
+      constructor
+      rfl
+    | assume HA HB IA IB =>
+      intro HΓΔ Hs;
+      rw [<-Hs]
+      constructor
+      apply IA
+      assumption
+      rfl
+      apply IB
+      constructor
+      assumption
+      constructor
+      constructor
+      rfl
+    | intersect HA HB IA IB => 
+      intro HΓΔ Hs;
+      rw [<-Hs]
+      constructor
+      apply IA
+      assumption
+      rfl
+      apply IB
+      constructor
+      assumption
+      constructor
+      constructor
+      rfl
+    | union HA HB IA IB => 
+      intro HΓΔ Hs;
+      rw [<-Hs]
+      constructor
+      apply IA
+      assumption
+      rfl
+      apply IB
+      constructor
+      assumption
+      constructor
+      constructor
+      rfl
+    | dand HA HB IA IB => 
+      intro HΓΔ Hs;
+      rw [<-Hs]
+      constructor
+      apply IA
+      assumption
+      rfl
+      apply IB
+      constructor
+      assumption
+      constructor
+      constructor
+      rfl
+    | or HA HB IA IB => 
+      intro HΓΔ Hs;
+      rw [<-Hs]
+      constructor
+      apply IA
+      assumption
+      rfl
+      apply IB
+      assumption
+      rfl
+    | dimplies HA HB IA IB => 
+      intro HΓΔ Hs;
+      rw [<-Hs]
+      constructor
+      apply IA
+      assumption
+      rfl
+      apply IB
+      constructor
+      assumption
+      constructor
+      constructor
+      rfl
+    | forall_ HA HB IA IB => 
+      intro HΓΔ Hs;
+      rw [<-Hs]
+      constructor
+      apply IA
+      assumption
+      rfl
+      apply IB
+      constructor
+      assumption
+      constructor
+      constructor
+      rfl
+    | exists_ HA HB IA IB => 
+      intro HΓΔ Hs;
+      rw [<-Hs]
+      constructor
+      apply IA
+      assumption
+      rfl
+      apply IB
+      constructor
+      assumption
+      constructor
+      constructor
+      rfl
+    | eq => sorry
+    | _ => intro HΓΔ Hs; first | contradiction | (repeat rw [<-Hs]; constructor)
+  }
+
+theorem HasType.downgrade {Γ: Context} {A s} (H: Γ.upgrade ⊢ A: sort s): Γ ⊢ A: sort s
+  := H.downgrade_helper Context.is_sub.upgrade rfl
